list & tree examples

src/ClConv2.v
@@ -1,5 +1,6 @@
 Require String Vector.
 Require Import List FunctionalExtensionality.
+Require Import StateMachines.Inhabit.
 Import ListNotations.
 Set Universe Polymorphism.
 Open Scope type_scope.
@@ -50,12 +51,29 @@ Definition rets_effect (e : effect) :=
 
 Inductive yield_effect := yield : yield_effect.
 
+Definition equiv_coro A B state (step : step_type (fun _:yield_effect => A)(fun _:yield_effect => B) state) init p :=
+  exists op s, forall r,
+      step init yield r = Some (s r, op r) /\ equiv' step (s r) (p r) (op r).
+
 Definition seqE A B (e : t (fun _:yield_effect => A) (fun _:yield_effect => B)) : (A -> (B -> t (fun _:yield_effect => A) (fun _:yield_effect => B)) -> t args_effect rets_effect) -> t args_effect rets_effect :=
   match e with
   | Done _ _ => fun _ => Done _ _
   | Eff _ a p => fun cont => cont a p
   end.
 
+Notation "'const_yield' A" :=
+  (fun _:yield_effect => A)
+    (at level 10).
+
+Definition coro_type A B state (_ : step_type (const_yield A) (const_yield B) state):= B -> t (const_yield A)(const_yield B).
+
+Definition proc_coro A B state (step : step_type (const_yield A)(const_yield B) state)(c : coro_type step) (x : B) : (A -> coro_type step -> t args_effect rets_effect) -> t args_effect rets_effect :=
+  seqE (c x).
+
+Definition Let_coroutine A B
+           (c : B -> t (fun _:yield_effect => A)(fun _:yield_effect => B)) p
+  : t args_effect rets_effect :=
+  p c.
 Notation "n <- 'getN' ; e" :=
   (Eff getNat (tt : args_effect getNat) (fun n : rets_effect getNat => e))
     (at level 100, right associativity).
@@ -69,7 +87,7 @@ Notation "'putStr' s ; e" :=
   (Eff putString s (fun _ => e))
     (at level 200).
 Notation "n <- 'resume' c $ x ; e" :=
-  (seqE (c x) (fun n c => e))
+  (proc_coro c x (fun n c => e))
     (at level 100, right associativity).
 Notation "v1 <- 'yield' v2 ; e" :=
   (Eff yield v2 (fun v1 => e))
@@ -155,7 +173,7 @@ Inductive equiv_parent A B :
            (steps : forall k : Fin.t n, step_type (fun _:yield_effect => A) (fun _:yield_effect => B) (Vector.nth states k))
            (step : step_type (fun _:yield_effect => A) (fun _:yield_effect => B) state') init g,
       equiv step init (c x) ->
-    (forall v cs c, f' cs v c = f v (Vector.cons _ c _  cs)) ->
+      (forall v cs c, f' cs v c = f v (Vector.cons _ c _  cs)) ->
       (forall v,
           equiv_parent _ (fun k : Fin.t (S n) =>
                           Fin.caseS' k (fun k => step_type (fun _:yield_effect => A)(fun _:yield_effect => B) (Vector.nth (Vector.cons _ state' _ states) k)) step (fun k' => steps k'))
@@ -164,7 +182,21 @@ Inductive equiv_parent A B :
     equiv_parent _ steps
         (fun cs => seqE (c x) (f' cs))
         (fun ss =>
-           seqE' (step init yield x) (fun s' v => g v (ss, s')) (Done _ _)).
+           seqE' (step init yield x) (fun s' v => g v (ss, s')) (Done _ _))
+| EPSpawnLet :
+    forall n (c : B -> t (fun _:yield_effect => A)(fun _:yield_effect => B)) f f' state' states
+           (steps : forall k : Fin.t n, step_type (fun _:yield_effect => A) (fun _:yield_effect => B) (Vector.nth states k))
+           (step : step_type (fun _:yield_effect => A) (fun _:yield_effect => B) state') init g,
+      equiv_coro step init c ->
+      (forall cs c0, f' cs c0 = f (Vector.cons _ c0 _ cs)) ->
+      (equiv_parent _ (fun k : Fin.t (S n) =>
+                         Fin.caseS' k (fun k => step_type (fun _:yield_effect => A)(fun _:yield_effect => B)(Vector.nth (Vector.cons _ state' _ states) k)) step (fun k' => steps k'))
+                    f
+                    g) ->
+      equiv_parent _ steps
+                   (fun cs => Let_coroutine c (f' cs))
+                   (fun ss  => g (ss, init)).
+
 
 Lemma equiv_parent_sum :
   forall A B C D n (states : Vector.t Type n) fa fb ga gb steps (x : A + B),
@@ -188,6 +220,28 @@ Lemma equiv_parent_nat_rect :
   forall A B n (states : Vector.t Type n) X Y f f0 g g0 steps
          (x : Vector.t (B -> t (fun _:yield_effect => A)(fun _:yield_effect => B)) n -> X)
          (y : fin_prod states -> Y) N,
+    (forall x y, @equiv_parent A B n states steps (fun cs => f cs (x cs)) (fun ss => g ss (y ss))) ->
+    (forall N,
+        (forall x y, @equiv_parent A B n states steps
+                      (fun cs => nat_rect (fun X => _) (f cs) (f0 cs) N (x cs))
+                      (fun ss => nat_rect (fun Y => _) (g ss) (g0 ss) N (y ss))) ->
+        (forall x y,
+            equiv_parent _ steps
+                         (fun cs => nat_rect _ (f cs) (f0 cs) (S N) (x cs))
+                         (fun ss => nat_rect _ (g ss) (g0 ss) (S N) (y ss)))) ->
+  @equiv_parent A B n states steps
+               (fun cs => nat_rect _ (f cs) (f0 cs) N (x cs))
+               (fun ss => nat_rect _ (g ss) (g0 ss) N (y ss)).
+Proof.
+  intros.
+  revert x y.
+  induction N; intros; (auto || simpl; auto).
+Qed.
+
+Lemma equiv_parent_nat_rect_dep :
+  forall A B N n (states : Vector.t Type n) X Y f f0 g g0 steps
+         (x : Vector.t (B -> t (fun _:yield_effect => A)(fun _:yield_effect => B)) n -> X)
+         (y : fin_prod states -> Y),
     (forall x y, @equiv_parent A B n states steps (fun cs => f cs (x cs)) (fun ss => g ss (y ss))) ->
     (forall N,
         (forall x y, @equiv_parent A B n states steps
@@ -239,7 +293,7 @@ Ltac curry_lhs' :=
     let rec aux p :=
         lazymatch p with
         | ?f (_,_) =>
-          let f' := open_constr:(prod_curry_rev (fun x => _)) in
+          let f' := open_constr:(prod_curry_rev (fun _ => _)) in
           unify f f'; unfold prod_curry_rev
         | ?p' _ =>
           aux p'
@@ -591,6 +645,11 @@ Ltac prog_eq :=
     let u := open_constr:(fun v ccs0 => _) in
     unify f u;
     apply eq_refl
+  | |- _ = ?f ?ccs =>
+    vec_replace ccs;
+    let u := open_constr:(fun ccs0 => _) in
+    unify f u;
+    apply eq_refl
   end.
 
 Ltac derive_parent_core :=
@@ -629,6 +688,7 @@ Definition ex_coroutine k n : t (fun _:yield_effect => nat) (fun _:yield_effect 
     _ <- yield (n + m)%nat;
     Done _ _.
 
+(*
 Definition ex N :=
   let c1 := ex_coroutine 2 in
   let c2 := ex_coroutine 3 in
@@ -641,7 +701,7 @@ Definition ex N :=
                   m2 <- resume c2 $ n2;
                   putN m2;
                   rec c1 c2) N c1 c2.
-
+*)
   
 Ltac derive_parent_fix :=
   lazymatch goal with
@@ -706,6 +766,7 @@ Proof.
   solve_child.
 Defined.
 
+(*
 Opaque seqE.
 Theorem ex_derive_parent :
   forall N, {g | @equiv_parent nat nat 0 (Vector.nil _)
@@ -716,11 +777,12 @@ Proof.
   unfold ex.
   intros.
   eexists.
-  repeat (solve_child || derive_parent).
+  repeat (eapply (proj2_sig (projT2 (projT2 (ex_coroutine_derive _ _)))) || derive_parent).
 Defined.
-Eval cbv -[nat_rect] in (fun N => proj1_sig (ex_derive_parent N)).
+Eval simpl in (fun N => proj1_sig (ex_derive_parent N)).
 
 Transparent seqE.
+*)
 
 Lemma equiv_parent_eq_general : forall A B n states steps f g,
     @equiv_parent A B n states steps f g ->
@@ -819,6 +881,24 @@ Proof.
   subst.
   simpl.
   auto.
+  unfold Let_coroutine.
+  rewrite H0.
+  apply IHequiv_parent.
+  intro k.
+  pattern k.
+  apply Fin.caseS'; simpl; intros.
+  destruct H as (op0,(s,(H5,H6))).
+  rewrite H5 in H4.
+  assert (op0 x = op) by congruence; assert (s x = next) by congruence; subst.
+  auto.
+  auto.
+  intro k.
+  pattern k.
+  apply Fin.caseS'; simpl; intros.
+  destruct H as (op0,(s,(H5,H6))).
+  rewrite H5 in H4.
+  congruence.
+  auto.
 Qed.
 
 Lemma equiv_parent_eq : forall A B states steps f g cs ss,
@@ -841,8 +921,6 @@ Ltac my_instantiate ev t :=
   pose ev as H;
   instantiate (1 := t) in (Value of H);
   subst H.
-
-Definition dummy (A:Type)(x:A) := True.
 
 Ltac st_op_to_ev :=
   lazymatch goal with
@@ -869,6 +947,7 @@ Ltac st_op_to_ev :=
     cbv beta
   end.
 
+(*
 Theorem ex_correct : forall N,
     ex N = proj1_sig (ex_derive_parent N) tt.
 Proof.
@@ -880,6 +959,7 @@ Proof.
   reflexivity.
   auto.
 Qed.
+ *)
 
 Lemma derive_parent_rect : forall state A N a0 f f0 st0 stS op0 opS step,
     (forall a, equiv' step (st0 a) (nat_rect (fun n => A -> _) (f a) (f0 a) 0 a) (op0 a)) ->
@@ -1106,10 +1186,14 @@ Ltac derive_rec env :=
   ].
 
 Ltac derive_child' env :=
-  match goal with
+  lazymatch goal with
     |- equiv _ _ ?x =>
     let y := eval red in x in
         change x with y
+  | |- equiv_coro _ _ ?x =>
+    let y := eval red in x in
+        change x with y
+  | _ => idtac
   end;
   simpl;
   match goal with
@@ -1119,9 +1203,60 @@ Ltac derive_child' env :=
   end;
   repeat eexists;
   [ dest_sum; simpl; unify_fun
-  | derive_core open_constr:(fun x => inr x) tt
+  | derive_core open_constr:(fun x => inr x) env
   ].
-  
+
+Lemma ex_coroutine_derive' :
+  { state & { step & forall k, { init | @equiv_coro _ _ state step init (ex_coroutine k) }}}.
+  do 3 eexists.
+  lazymatch goal with
+    |- equiv _ _ ?x =>
+    let y := eval red in x in
+        change x with y
+  | |- equiv_coro _ _ ?x =>
+    let y := eval red in x in
+        change x with y
+  end;
+  simpl;
+  match goal with
+    |- _ _ ?init _ =>
+    let u := open_constr:(inl (tt,k)) in
+    unify init u
+  end.
+  repeat eexists.
+  match goal with
+    |- _ (@inl ?A ?B _) _ _ = _ (?s _, _) =>
+    let u := open_constr:(_+_) in
+    unify B u;
+    let u := open_constr:(fun x => inr (inl (tt,k,x))) in
+    unify s u
+  end.
+  all: swap 1 2.
+  cbv beta.
+  derive_core open_constr:(fun x => inr x) (tt,k,r).  
+  simpl.
+  pattern_rhs r.
+  apply equal_f.
+  pattern_rhs yield.
+  apply equal_f.
+  curry_lhs.
+  unify_fun.
+  Grab Existential Variables.
+  2: exact unit.
+  intros.
+  exact None.
+Defined.
+
+Definition ex_coroutine_equiv k : equiv_coro _ _ (ex_coroutine k) :=
+  proj2_sig (projT2 (projT2 ex_coroutine_derive') k).
+
+Definition ex_coroutine_equiv' k
+  : equiv_coro ltac:(let x := eval simpl in (projT1 (projT2 ex_coroutine_derive')) in exact x) ltac:(let x := eval simpl in (proj1_sig (projT2 (projT2 ex_coroutine_derive') k)) in exact x) (ex_coroutine k) :=
+  ex_coroutine_equiv k.
+
+Hint Resolve ex_coroutine_equiv ex_coroutine_equiv' : equivc.
+
+(*
 Theorem ex_derive :
   {state & {step & forall N, {init | @equiv _ _ _ state step init (ex N)}}}.
 Proof.
@@ -1153,8 +1288,8 @@ Definition ex2 : t args_effect rets_effect :=
     | inl n => putN n; Done _ _
     | inr _ => Done _ _
     end.
+*)
 
-Opaque seqE.
 (*
 Theorem ex2_derive_parent :
   {g | @equiv_parent _ _ 0 (Vector.nil _)
@@ -1167,7 +1302,8 @@ Proof.
   unshelve (repeat (intros; (derive_child' tt || derive_parent)));
   exact (fun _ _ _ => None) ||
   exact unit.
-Defined.*)
+Defined.
+*)
 
 Ltac derive env :=
   eexists;
@@ -1198,31 +1334,1040 @@ Ltac derive env :=
     apply eq_refl || (pattern_rhs tt; apply eq_refl)
   ].
 
+(*
 Theorem ex2_derive :
   { state & { step & { init | @equiv _ _ _ state step init ex2 } } }.
 Proof.
   unshelve derive tt; simpl; intros; (exact None || exact unit || exact tt).
 Defined.
 
-Inductive deposit_or_tock (A B : Type) :=
-  Start : t (fun _:yield_effect => A)(fun _:yield_effect => B) -> deposit_or_tock A B
-| Tock : nat -> deposit_or_tock A B.
+Eval cbv in projT1 (projT2 ex2_derive).
+ *)
 
-Fixpoint always_tock_0 A B (shep : deposit_or_tock A B -> t (fun _:yield_effect => unit)(fun _:yield_effect => deposit_or_tock A B)) fuel :=
-  match fuel with
-  | O => Done _ _
-  | S n' =>
-    c <- resume shep $ (Tock _ _ 0);
-      always_tock_0 shep n'
+Definition replace A i l (a:A) :=
+  (fix aux i l pre :=
+    match l with
+    | [] => []
+    | x::l' =>
+      match i with
+      | O => pre ++ a :: l'
+      | S i' => aux i' l' (pre ++ [x])
+      end
+    end) i l [].
+
+Definition pipe A B (a : A)(f : A -> B) := f a.
+
+
+Definition option_branch A B (f : A -> B) f0 o :=
+  match o with
+  | None => f0
+  | Some a => f a
   end.
 
-Definition shephard A B fuel (rq : deposit_or_tock A B) :=
-  fix aux inprogress fuel :=
-    match fuel with
-    | O => Done
-    | S fuel' =>
-      match rq with
-      | Start coro =>
-        aux (coro::inprogrss) fuel'
-      | Tock i =>
-        nth i inprogress 
+Definition nat_rect_nondep A f (f0 : nat -> A -> A) :=
+  fix F (n : nat) : A :=
+    match n with
+    | O => f
+    | S n' => f0 n' (F n')
+    end.
+
+Instance coro_type_inhabitant A B state step :
+  Inhabit (@coro_type A B state step) :=
+  { inhabitant := fun _ => Done _ _ }.
+
+Instance prod_inhabitant A B `{IA : Inhabit A} `{IB : Inhabit B} : Inhabit (A * B) :=
+  { inhabitant := (inhabitant, inhabitant) }.
+
+Instance unit_inhabitant : Inhabit unit := {inhabitant := tt }.
+
+Instance sum_inhabitant A B `{IA : Inhabit A} : Inhabit (A + B) :=
+  { inhabitant := inl inhabitant }.
+
+Instance arrow_inhabitant A B `{IB : Inhabit B} : Inhabit (A -> B) :=
+  { inhabitant := fun _:A => inhabitant }.
+
+Instance option_inhabitant A : Inhabit (option A) :=
+  { inhabitant := None }.
+
+Instance t_inhabitant e a r : Inhabit (@t e a r) :=
+  { inhabitant := Done _ _ }.
+
+Definition seq_abs A B state (step : step_type (fun _:yield_effect => A)(fun _:yield_effect => B) state) (x:B) C (_:C) (g : A -> C -> t args_effect rets_effect) := t_inhabitant.
+
+Definition step_state A B state (step : step_type (fun _:yield_effect => A)(fun _:yield_effect => B) state) st x g :=
+  seqE' (step st yield x) (fun s v => g v s) (Done _ _).
+
+Opaque dummy.
+
+Definition K A B :=
+  fun (x : A)(_ : B) => x.
+
+Ltac get_init c :=
+  let init := open_constr:(_) in
+  let _ := constr:(ltac:(auto with equivc) : equiv_coro _ init c) in
+  init.
+
+Ltac to_dummy i p :=
+  lazymatch p with
+  | pipe ?c ?f =>
+    let init := get_init c in
+    let x := (eval cbv beta in (f (dummy _ _ i))) in
+    let d := to_dummy (S i) x in
+    lazymatch d with
+    | context [dummy _ ?T i] =>
+      lazymatch (eval pattern (dummy _ T i) in d) with
+      | ?g _ =>
+        constr:((pipe, init, g))
+      end
+    end
+  | @Eff _ args_effect rets_effect ?e ?a ?f =>
+    let x := (eval cbv beta in (f (dummy _ _ i))) in
+    let d := to_dummy (S i) x in
+    lazymatch (eval pattern (dummy _ (rets_effect e) i) in d) with
+    | ?g _ =>
+      constr:((@Eff _ args_effect rets_effect e a, g))
+    end
+  | @proc_coro ?A ?B ?state ?step ?c ?z ?f =>
+    let x := (eval cbv beta in (f (dummy _ _ i) (dummy _ _ (S i)))) in
+    lazymatch f with
+    | context [proc_coro] =>
+      let d := to_dummy (S (S i)) x in
+      lazymatch type of f with
+      | _ -> ?T -> _ =>
+        lazymatch (eval pattern (dummy _ A i), (dummy _ T (S i)) in d) with
+        | ?g _ _ =>
+          constr:((@seq_abs A B state step z (coro_type step) c, g))
+        end
+      end
+    | _ =>
+      constr:((@seq_abs A B state step z (coro_type step) c, f))
+    end
+  | @option_branch ?A ?B ?f ?f0 ?o =>
+    let x := (eval cbv beta in (f (dummy _ _ i))) in
+    let d := to_dummy (S i) x in
+    let d0 := to_dummy i f0 in
+    lazymatch (eval pattern (dummy _ A i) in d) with
+    | ?g _ =>
+      constr:((@option_branch A B, g : A -> _, d0, o))
+    end
+  | @nat_rect_nondep ?A ?f ?f0 ?n ?a =>
+    let x := (eval cbv beta in (f0 (dummy _ _ i) (dummy _ _ (S i)) (dummy _ _ (S (S i))))) in
+    let y := (eval cbv beta in (f (dummy _ _ i))) in
+    let d := to_dummy (S i) y in
+    let d0 := to_dummy (S (S (S i))) x in
+    let T := type of a in
+    lazymatch (eval pattern (dummy _ nat i), (dummy _ A (S i)), (dummy _ T (S (S i))) in d0) with
+    | ?g0 _ _ _ =>
+      lazymatch (eval pattern (dummy _ T i) in d) with
+      | ?g _ =>
+        constr:((@nat_rect_nondep A, g, g0, n, a))
+      end
+    end
+  | _ => p
+  end.
+
+Ltac reconstruct tree :=
+  lazymatch tree with
+  | (pipe, ?init, ?f) =>
+    let x := (eval cbv beta in (f init)) in
+    reconstruct x
+  | (Eff ?e ?a, ?p) =>
+    let x := (eval cbv beta in (p (dummy _ _ tt))) in
+    let p' := reconstruct x in
+    lazymatch type of p with
+    | ?ty -> _ =>
+      lazymatch (eval pattern (dummy _ ty tt) in p') with
+      | ?p'' _ =>
+        constr:(Eff e a p'')
+      end
+    end
+  | (@seq_abs ?A ?B _ ?step ?z ?state ?st, ?p) =>
+    let x := (eval cbv beta in (p (dummy _ _ tt) (dummy _ _ tt))) in
+    let p' := reconstruct x in
+    lazymatch (eval pattern (dummy _ A tt), (dummy _ state tt) in p') with
+    | ?p'' _ _ =>
+      constr:(@step_state A B _ step st z p'')
+    end
+  | (@option_branch ?A ?B, ?f, ?f0, ?o) =>
+    let x := (eval cbv beta in (f (dummy _ _ tt))) in
+    let p' := reconstruct x in
+    lazymatch (eval pattern (dummy _ A tt) in p') with
+    | ?p'' _ =>
+      constr:(@option_branch A B p'' f0 o)
+    end
+  | (@nat_rect_nondep ?A, ?f, ?f0, ?n, ?a) =>
+    let x := (eval cbv beta in (f (dummy _ _ tt))) in
+    let y := (eval cbv beta in (f0 (dummy _ _ tt) (dummy _ _ tt) (dummy _ _ tt))) in
+    let f' := reconstruct x in
+    let f0' := reconstruct y in
+    let ty := type of a in
+    lazymatch (eval pattern (dummy _ ty tt) in f') with
+    | ?f'' _ =>
+      lazymatch (eval pattern (dummy _ nat tt), (dummy _ A tt), (dummy _ ty tt) in f0') with
+      | ?f0'' _ _ _ =>
+        constr:(@nat_rect_nondep A f'' f0'' n a)
+      end
+    end
+  | _ => tree
+  end.
+
+Ltac coro_to_state p :=
+  let x := to_dummy 0 p in
+  lazymatch x with
+  | context [@coro_type _ _ ?state ?step] =>
+    lazymatch (eval pattern (coro_type step) in x) with
+    | ?F _ =>
+      let y := (eval cbv beta in (F state)) in
+      reconstruct y
+    end
+  end.
+
+(*
+Definition take_nth n :=
+  pipe (ex_coroutine 0 : coro_type (projT1 (projT2 ex_coroutine_derive')))
+       (fun c0 =>
+          pipe (ex_coroutine 1 : coro_type (projT1 (projT2 ex_coroutine_derive')))
+               (fun c1 =>
+                  nth_error [c0; c1] n)).
+
+
+Goal nat -> True.
+  intro n.
+  let x := (eval red in (take_nth n)) in
+  let x' := coro_to_state x in
+  idtac x'.
+Abort.
+
+
+Definition take_nth_get (g : forall A, A -> t args_effect rets_effect) :=
+  pipe (ex_coroutine 0 : coro_type (projT1 (projT2 ex_coroutine_derive')))
+       (fun c0 =>
+          n <- getN;
+          pipe (ex_coroutine 1 : coro_type (projT1 (projT2 ex_coroutine_derive')))
+               (fun c1 =>
+
+                  g _ (nth_error [c0; c1] n))).
+
+Goal (forall A, A -> t args_effect rets_effect) -> True.
+  intro g.
+  let x := (eval red in (take_nth_get g)) in
+  let x' := coro_to_state x in
+  idtac x'.
+Abort.
+
+Definition opt_nth (n:nat)(g : forall A, A  -> t args_effect rets_effect) :=
+  pipe (ex_coroutine 0 : coro_type (projT1 (projT2 ex_coroutine_derive')))
+       (fun c0 =>
+          pipe (ex_coroutine 1 : coro_type (projT1 (projT2 ex_coroutine_derive')))
+               (fun c1 =>
+                  n <- getN;
+                  option_branch
+                    (fun c => g _ c)
+                    (Done _ _)
+                    (nth_error [c0; c1] n))).
+
+Goal nat -> (forall A, A -> t args_effect rets_effect) -> True.
+  intros n g.
+  let x := (eval red in (opt_nth n g)) in
+  let x' := coro_to_state x in
+  idtac x'.
+Abort.
+
+*)
+
+Definition proc_ex k :=
+  pipe (ex_coroutine 0 : coro_type (projT1 (projT2 ex_coroutine_derive')))
+       (fun c =>
+          r <- resume c $ k;
+            putN r; Done _ _).
+Goal nat -> True.
+  intro k.
+  let x := (eval red in (proc_ex k)) in
+  let x' := coro_to_state x in
+  idtac x'.
+Abort.
+
+Definition opt_nth' (n:nat) :=
+  pipe (ex_coroutine 0 : coro_type (projT1 (projT2 ex_coroutine_derive')))
+       (fun c0 =>
+          pipe (ex_coroutine 1 : coro_type (projT1 (projT2 ex_coroutine_derive')))
+               (fun c1 =>
+                  n <- getN;
+                    option_branch
+                      (fun c : @coro_type nat nat _ _ =>
+                         r <- resume c $ 2;
+                           putN r; Done _ _)
+                      (Done _ _)
+                      (nth_error [c0; c1] n))).
+
+Goal nat -> True.
+  intros n.
+  let x := (eval red in (opt_nth' n)) in
+  let x' := coro_to_state x in
+  idtac x'.
+Abort.
+
+Fixpoint zip_list A1 A2 (l1 : list A1)(l2 : list A2) : option (list (A1 * A2)):=
+  match l1, l2 with
+  | [], [] => Some []
+  | a1::l1', a2::l2' =>
+    option_map (fun l => (a1,a2) :: l) (zip_list l1' l2')
+  | _, _ => None
+  end.
+
+Class Foldable (F : Type -> Type) :=
+  { foldr : forall A B, (A -> B -> B) -> B -> F A -> B;
+    zip : forall A1 A2, F A1 -> F A2 -> option (F (A1 * A2));
+    to_list : forall A, F A -> list A;
+    to_list_foldr : forall A B (f : A -> B -> B) b x,
+        foldr f b x = fold_right f b (to_list x);
+    zip_to_list : forall A1 A2 (x1 : F A1)(x2 : F A2) x,
+        zip x1 x2 = Some x -> Some (to_list x) = zip_list (to_list x1) (to_list x2)
+  }.
+
+Program Instance list_Foldable : Foldable list :=
+  { foldr := fun A B => @fold_right B A;
+    zip := zip_list;
+    to_list := fun _ x => x
+  }.
+
+Definition size A F `{F_Foldable : Foldable F} (x : F A) : (nat : Type) :=
+  foldr (fun _ accum => S accum) 0 x.
+
+Definition nth_err A F `{F_Foldable : Foldable F}(x : F A) :=
+  foldr (fun a p n =>
+           match n with
+           | O => Some a
+           | S n' => p n'
+           end)
+        (fun _ => None) x.
+
+Definition GenForall2 A1 A2 F `{F_Foldable : Foldable F}
+           (R : A1 -> A2 -> Prop) (x1 : F A1) (x2 : F A2) :=
+  exists x, zip _ _ x1 x2 = Some x /\ foldr (fun '(a1, a2) p => R a1 a2 /\ p) True x.
+
+Lemma GenForall2_cons : forall A1 A2 (R : A1 -> A2 -> Prop) (x1 : list A1) (x2 : list A2) a1 a2,
+    R a1 a2 ->
+    GenForall2 R x1 x2 ->
+    GenForall2 R (a1::x1) (a2::x2).
+Proof.
+  unfold GenForall2. simpl.
+  intros.
+  destruct H0 as (x,(H1,H2)).
+  exists ((a1,a2) :: x).
+  split.
+  rewrite H1.
+  auto.
+  simpl.
+  auto.
+Qed.
+
+Lemma nth_err_nth_error : forall A F (F_Foldable : Foldable F) (x : F A) n,
+    nth_err _ x n = nth_error (to_list _ x) n.
+Proof.
+  intros.
+  unfold nth_err.
+  rewrite to_list_foldr.
+  revert n.
+  induction (to_list A x); intros; simpl.
+  destruct n; auto.
+  destruct n; simpl; auto.
+Qed.
+
+Lemma size_length : forall A F (F_Foldable : Foldable F) (x : F A),
+    size _ x = length (to_list _ x).
+Proof.
+  intros.
+  unfold size.
+  rewrite to_list_foldr.
+  induction (to_list _ x); simpl; auto.
+Qed.
+
+Lemma nth_err_Some : forall A (F : Type -> Type) (F_Foldable : Foldable F) (x : F A) n a,
+    nth_err _ x n = Some a ->
+    n < size _ x.
+Proof.
+  intros.
+  unfold size, nth_err in *.
+  rewrite to_list_foldr in *.
+  revert n a H.
+  induction (to_list _ x); simpl; intros.
+  congruence.
+  destruct n.
+  auto with arith.
+  apply -> PeanoNat.Nat.succ_lt_mono.
+  eauto.
+Qed.
+
+Lemma nth_err_None : forall A F (F_Foldable : Foldable F) (x : F A) n,
+    nth_err _ x n = None ->
+    ~ n < size _ x.
+Proof.
+  intros.
+  unfold size, nth_err in *.
+  rewrite to_list_foldr in *.
+  revert n H.
+  induction (to_list _ x); simpl; intros.
+  auto with arith.
+  destruct n.
+  congruence.
+  apply IHl in H.
+  auto with arith.
+Qed.
+(*
+Lemma GenForall2_size : forall A1 A2 F (F_Foldable : Foldable F) R (x1 : F A1) (x2 : F A2),
+    GenForall2 R x1 x2 -> size _ x1 = size _ x2.
+Proof.
+  intros.
+  destruct H.
+  auto.
+Qed.
+*)
+Lemma GenForall2_Forall2 : forall A1 A2 F (F_Foldable : Foldable F) R (x1 : F A1) (x2 : F A2),
+    GenForall2 R x1 x2 -> Forall2 R (to_list _ x1) (to_list _ x2).
+Proof.
+  intros.
+  unfold GenForall2 in H.
+  destruct H as (x,(H0,H1)).
+  rewrite to_list_foldr in H1.
+  apply zip_to_list in H0.
+  generalize dependent (to_list _ x).
+  generalize (to_list A2 x2).
+  induction (to_list _ x1); intros.
+  destruct l.
+  auto.
+  simpl in H0.
+  congruence.
+  destruct l0.
+  simpl in H0.
+  congruence.
+  simpl in *.
+  destruct (zip_list l l0) eqn:?.
+  simpl in *.
+  symmetry in Heqo.
+  inversion H0. subst.
+  simpl in H1.
+  econstructor.
+  tauto.
+  apply IHl in Heqo.
+  auto.
+  tauto.
+  simpl in H0.
+  congruence.
+Qed.
+
+Lemma GenForall2_size : forall (A1 A2 : Type) (F : Type -> Type) (F_Foldable : Foldable F) R (x1 : F A1) (x2 : F A2),
+    GenForall2 R x1 x2 ->
+    size _ x1 = size _ x2.
+Proof.
+  intros.
+  destruct H.
+  destruct H.
+  apply zip_to_list in H.
+  unfold size.
+  repeat rewrite to_list_foldr in *.
+  generalize dependent (to_list _ x2).
+  generalize dependent (to_list _ x).
+  induction (to_list _ x1); simpl in *; intros.
+  destruct l0; simpl in *; congruence.
+  destruct l1; simpl in *.
+  congruence.
+  f_equal.
+  destruct (zip_list l l1) eqn:?; simpl in *.
+  apply (IHl l2).
+  inversion H. subst.
+  simpl in H0.
+  tauto.
+  inversion H. subst.
+  auto.
+  congruence.
+Qed.
+
+Lemma GenForall2_nth_Some_None : forall (A1 A2 : Type) (F : Type -> Type) (F_Foldable : Foldable F) R (x1 : F A1) (x2 : F A2) n a1,
+    GenForall2 R x1 x2 ->
+    nth_err _ x1 n = Some a1 ->
+    nth_err _ x2 n = None ->
+    False.
+Proof.
+  intros.
+  apply nth_err_None in H1.
+  apply nth_err_Some in H0.
+  apply GenForall2_size in H.
+  rewrite H in H0.
+  auto.
+Qed.
+
+Lemma GenForall2_nth_None_Some : forall (A1 A2 : Type) (F : Type -> Type) (F_Foldable : Foldable F) R (x1 : F A1) (x2 : F A2) n a2,
+    GenForall2 R x1 x2 ->
+    nth_err _ x1 n = None ->
+    nth_err _ x2 n = Some a2 ->
+    False.
+Proof.
+  intros.
+  apply nth_err_Some in H1.
+  apply nth_err_None in H0.
+  apply GenForall2_size in H.
+  rewrite H in H0.
+  auto.
+Qed.
+
+Lemma GenForall2_nth_Some : forall (A1 A2 : Type) (F : Type -> Type) (F_Foldable : Foldable F) R (x1 : F A1) (x2 : F A2) n a1 a2,
+    GenForall2 R x1 x2 ->
+    nth_err _ x1 n = Some a1 ->
+    nth_err _ x2 n = Some a2 ->
+    R a1 a2.
+Proof.
+  intros.
+  unfold nth_err in *.
+  unfold GenForall2 in H.
+  destruct H.
+  destruct H.
+  unfold size in H.
+  rewrite to_list_foldr in H2.
+  rewrite to_list_foldr in H0.
+  rewrite to_list_foldr in H1.
+  apply zip_to_list in H.
+  generalize dependent (to_list _ x2).
+  generalize dependent (to_list _ x).
+  revert n a1 a2 H0.
+  induction (to_list _ x1); simpl in *; intros.
+  destruct l0.
+  inversion H. subst.
+  simpl in H1.
+  congruence.
+  congruence.
+  destruct l1; [congruence|].
+  destruct (zip_list l l1) eqn:?; simpl in *; [|congruence].
+  inversion H. subst.
+  simpl in H2.
+  destruct n.
+  inversion H0. subst.
+  inversion H1. subst.
+  tauto.
+  destruct H2.
+  eapply IHl.
+  eauto.
+  eauto.
+  symmetry. eauto.
+  auto.
+Qed.
+
+Hint Resolve GenForall2_size nth_err_None nth_err_Some GenForall2_cons GenForall2_nth_None_Some GenForall2_nth_Some_None : foldable.
+Transparent proc_coro.
+
+
+Definition loop_ex (n i : nat)(g : forall A, A -> t args_effect rets_effect) :=
+  pipe (ex_coroutine 0 : coro_type (projT1 (projT2 ex_coroutine_derive')))
+       (fun c0 =>
+          nat_rect_nondep
+            (fun l => option_branch
+                        (fun c => g _ c)
+                        (Done _ _)
+                        (nth_err _ l i))
+            (fun m rec l =>
+               pipe (ex_coroutine m : coro_type (projT1 (projT2 ex_coroutine_derive')))
+                    (fun cm =>
+                       rec (cm::l)))
+            n [c0]).
+
+Definition equiv_coro' A B `{IA : Inhabit A} `{IB : Inhabit B} state (step : step_type _ _ state) st (coro : B -> t (const_yield A) (const_yield B)) :=
+  exists op, equiv' step st (r <- yield inhabitant; coro r) op.
+
+Ltac get_step c :=
+  let step := open_constr:(_) in
+  let _ := constr:(ltac:(auto with equivc') : equiv_coro' step _ c) in
+  step.
+
+Ltac derive_child'' env :=
+  lazymatch goal with
+    |- equiv _ _ ?x =>
+    let y := eval red in x in
+        change x with y
+  | |- equiv_coro' _ _ ?x =>
+    let y := eval red in x in
+        change x with y
+  | _ => idtac
+  end;
+  simpl;
+  match goal with
+    |- _ _ ?init _ =>
+    let u := open_constr:(inl env) in
+    unify init u
+  end;
+  let r := fresh in
+  repeat eexists; try econstructor;
+  [ intro r; derive_core open_constr:(fun x => inr x) (env,r)
+  | intros; dest_step'
+  ].
+
+Lemma ex_coroutine_derive'' :
+  { state & { step & forall k, { init | @equiv_coro' _ _ _ _ state step init (ex_coroutine k) }}}.
+  do 3 eexists.
+  derive_child'' (tt,k).
+  Grab Existential Variables.
+  2: exact unit.
+  intros.
+  exact None.
+Defined.
+
+Definition ex_coroutine_equiv2 k : equiv_coro' _ _ (ex_coroutine k) :=
+  proj2_sig (projT2 (projT2 ex_coroutine_derive'') k).
+
+Definition ex_coroutine_equiv2' k
+  : equiv_coro' ltac:(let x := eval simpl in (projT1 (projT2 ex_coroutine_derive'')) in exact x) ltac:(let x := eval simpl in (proj1_sig (projT2 (projT2 ex_coroutine_derive'') k)) in exact x) (ex_coroutine k) :=
+  ex_coroutine_equiv2 k.
+
+Hint Resolve ex_coroutine_equiv2 ex_coroutine_equiv2' : equivc.
+Hint Resolve ex_coroutine_equiv2 : equivc'.
+
+Lemma GenForall2_nth_Some_equiv_coro : forall A B (IA : Inhabit A) (IB : Inhabit B) state (step : step_type (const_yield A) (const_yield B) state) F (F_Foldable : Foldable F) x1 x2 n a1 a2,
+    GenForall2 (fun (coro : coro_type step) (st : state) => equiv_coro' step st coro) x1 x2 ->
+    nth_err _ x1 n = Some a1 ->
+    nth_err _ x2 n = Some a2 ->
+    equiv_coro' step a2 a1.
+Proof.
+  intros.
+  eapply (GenForall2_nth_Some (R := (fun (coro : coro_type step) (st : state) => equiv_coro' step st coro))); eauto.
+Qed.
+
+Hint Resolve GenForall2_nth_Some_equiv_coro : foldable.
+
+Ltac generalize_and_ind :=
+  lazymatch goal with
+    |- nat_rect_nondep ?A _ ?k ?l = nat_rect_nondep _ _ _ ?l' =>
+    lazymatch type of l with
+    | context [@coro_type _ _ ?state ?step] =>
+        cut (GenForall2 (fun (coro : coro_type step) (st : state) => equiv_coro' step st coro) l l');
+      [ generalize l l'
+       |unfold GenForall2; eexists; split; [reflexivity|simpl; eauto with equivc]];
+      induction k; intros; unfold nat_rect_nondep
+    end
+  end.
+
+
+Ltac proc_step :=
+  lazymatch goal with
+    |- proc_coro ?c ?x ?f = step_state ?step ?st _ ?g =>
+    let H := fresh in
+    let H0 := fresh in
+    assert (equiv_coro' step st c) as (H,H0);
+    [eauto with foldable
+    |
+    let s := fresh "s" in
+    let e := fresh "e" in
+    let a := fresh "a" in
+    let p := fresh "p" in
+    let next := fresh "next" in
+    let op := fresh "op" in
+    let H1 := fresh in
+    let H2 := fresh in
+    inversion H0 as [s e a p next op H1 H2|]; subst;
+    unfold step_state at 1, seqE' at 1;
+    rewrite H2;
+    lazymatch goal with
+      |- context [match op ?x with _ => _ end] =>
+      specialize (H1 x);
+      destruct (op x);
+      inversion H1; subst;
+      unfold proc_coro at 1, seqE at 1;
+      lazymatch goal with
+        H_ : _ = c x |- _ =>
+        rewrite <- H_
+      end
+    end
+    ]
+  end.
+
+Ltac dest_opt :=
+  lazymatch goal with
+    |- option_branch _ _ ?o = option_branch _ _ ?o0 =>
+    destruct o eqn:?, o0 eqn:?;
+             unfold option_branch
+  end.
+
+(*
+Notation "'let_coro' x := c 'in' p" :=
+  (pipe (c : coro_type ltac:(let step := get_step c in exact step))
+        (fun x => p))
+    (at level 200, only parsing).
+*)
+
+Definition loop_ex' (n i : nat) :=
+  pipe (ex_coroutine 0 : coro_type ltac:(let step := get_step (ex_coroutine 0) in exact step))
+       (fun c0 =>
+          nat_rect_nondep
+            (fun l => option_branch
+                        (fun c : @coro_type nat nat _ _=>
+                           r <- resume c $ 1;
+                             putN r;
+                             Done _ _)
+                        (Done _ _)
+                        (nth_err _ l i))
+            (fun m rec l =>
+               pipe (ex_coroutine m : @coro_type nat nat _ _)
+                    (fun cm =>
+                       rec (cm::l)))
+          n [c0]).
+
+Lemma loop_ex'_eq k n :
+  loop_ex' k n =
+  ltac:(let x := (eval red in (loop_ex' k n)) in
+        let x' := coro_to_state x in exact x').
+Proof.
+  unfold loop_ex'.
+  unfold pipe.
+  generalize_and_ind.
+  - dest_opt.
+    repeat (reflexivity || proc_step).
+    exfalso. eauto with foldable.
+    exfalso. eauto with foldable.
+    reflexivity.
+  - apply IHk.
+    apply GenForall2_cons; simpl in *; eauto with equivc.
+Qed.
+
+Inductive tree A := Node : A -> tree A -> tree A -> tree A | Leaf.
+Instance tree_Inhabit A : Inhabit (tree A) :=
+  { inhabitant := Leaf _ }.
+
+Fixpoint insert A x a0 (t : tree (nat * A)) :=
+  match t with
+  | Node (y,a) l r =>
+    if Nat.leb x y then
+      Node (y,a) (insert x a0 l) r
+    else
+      Node (y,a) l (insert x a0 r)
+  | Leaf _ =>
+    Node (x,a0) (Leaf _) (Leaf _)
+  end.
+
+Fixpoint bsearch A key (t : tree (nat * A)) :=
+  match t with
+  | Node (x,a) l r =>
+    match Nat.compare key x with
+    | Eq => Some a
+    | Lt => bsearch key l
+    | Gt => bsearch key r
+    end
+  | Leaf _ => None
+  end.
+
+Fixpoint replace_map A key a0 (t : tree (nat * A)) :=
+  match t with
+  | Node (x,a) l r =>
+    match Nat.compare key x with
+    | Eq => Node (key,a0) l r
+    | Lt => Node (x,a) (replace_map key a0 l) r
+    | Gt => Node (x,a) l (replace_map key a0 r)
+    end
+  | Leaf _ => Leaf _
+  end.
+
+Fixpoint foldr_map A B (f : A -> B -> B)(init : B)(t : tree (nat * A)) :=
+  match t with
+  | Node (k,a) l r => foldr_map f (f a (foldr_map f init r)) l
+  | Leaf _ => init
+  end.
+Require Import Arith.
+Fixpoint zip_map A1 A2 (m1 : tree (nat * A1))(m2 : tree (nat * A2)) :=
+  match m1, m2 with
+  | Node (k1,a1) l1 r1, Node (k2,a2) l2 r2 =>
+    if Nat.eq_dec k1 k2 then
+      match zip_map l1 l2, zip_map r1 r2 with
+      | Some ml, Some mr =>
+        Some (Node (k1, (a1,a2)) ml mr)
+      | _,_ => None
+      end
+    else
+      None
+  | Leaf _, Leaf _ => Some (Leaf _)
+  | _, _ => None
+  end.
+
+Definition from_map_to_list A (t : tree (nat * A)) :=
+  foldr_map (fun a accum => a :: accum) [] t.
+
+Lemma fold_right_cons_app : forall A (l l0 : list A),
+    fold_right (fun a l' => a::l') l0 l = l ++ l0.
+Proof.
+  induction l; simpl; intros; congruence.
+Qed.
+
+Program Instance map_Foldable : Foldable (fun A => tree (nat * A)) :=
+  { foldr := foldr_map;
+    zip := zip_map;
+    to_list := from_map_to_list
+  }.
+Next Obligation.
+  intros.
+  unfold from_map_to_list.
+  revert B f b;
+  induction x; simpl in *; intros.
+  rewrite IHx2.
+  destruct a.
+  rewrite IHx1.
+  rewrite IHx1.
+  replace (f a
+       (fold_right f b
+                   (foldr_map (fun (a0 : A) (accum : list A) => a0 :: accum) [] x2)))
+  with (fold_right f b (a :: foldr_map (fun a0 accum => a0 :: accum) [] x2)) by auto.
+  rewrite <- fold_right_app.
+  f_equal.
+  setoid_rewrite IHx1 at 2.
+  setoid_rewrite IHx2 at 2.
+  replace ((a
+     :: fold_right (fun (a0 : A) (accum : list A) => a0 :: accum) []
+     (foldr_map (fun (a0 : A) (accum : list A) => a0 :: accum) [] x2)))
+  with (fold_right (fun (a0 : A) (accum : list A) => a0 :: accum) []
+                   (a ::foldr_map (fun (a0 : A) (accum : list A) => a0 :: accum) [] x2)) by auto.
+  rewrite <- fold_right_app.
+  rewrite fold_right_cons_app.
+  rewrite fold_right_cons_app.
+  do 2 rewrite app_nil_r.
+  auto.
+  auto.
+Qed.
+Next Obligation.
+  unfold from_map_to_list.
+  enough (forall l1 l2 l, zip_list l1 l2 = Some l ->
+                          Some
+    (foldr_map (fun (a : A1 * A2) (accum : list (A1 * A2)) => a :: accum) l x) =
+  zip_list (foldr_map (fun (a : A1) (accum : list A1) => a :: accum) l1 x1)
+    (foldr_map (fun (a : A2) (accum : list A2) => a :: accum) l2 x2)) by auto.
+  revert x x2 H.
+  induction x1; simpl in *; intros.
+  destruct a.
+  destruct x2; simpl in *; [|congruence].
+  destruct p.
+  destruct (Nat.eq_dec n n0); [|congruence].
+  subst.
+  destruct (zip_map x1_1 x2_1) eqn:?; simpl in *; [|congruence].
+  destruct (zip_map x1_2 x2_2) eqn:?; simpl in *; [|congruence].
+  inversion H. subst.
+  simpl.
+  eapply IHx1_1 in Heqo.
+  rewrite <- Heqo.
+  reflexivity.
+  simpl.
+  eapply IHx1_2 in Heqo0.
+  rewrite <- Heqo0.
+  simpl.
+  reflexivity.
+  auto.
+  destruct x2; [congruence|].
+  inversion H. subst.
+  auto.
+Qed.
+
+Lemma GenForall2_bsearch_Some_None : forall A1 A2 (R : A1 -> A2 -> Prop) m1 m2 k a,
+    GenForall2 R m1 m2 ->
+    bsearch k m1 = Some a ->
+    bsearch k m2 = None ->
+    False.
+Proof.
+  intros.
+  destruct H. destruct H.
+  clear H2.
+  revert x m2 H H1.
+  induction m1; intros; simpl in *.
+  destruct a0.
+  destruct m2.
+  destruct p.
+  simpl in H1.
+  destruct (k ?= n0) eqn:?.
+  congruence.
+  destruct (Nat.eq_dec n n0); [|congruence].
+  subst.
+  rewrite Heqc in H0.
+  destruct (zip_map m1_1 m2_1) eqn:?; [|congruence].
+  eauto.
+  destruct (Nat.eq_dec n n0); [|congruence].
+  subst.
+  rewrite Heqc in H0.
+  destruct (zip_map m1_1 m2_1) eqn:?; [|congruence].
+  destruct (zip_map m1_2 m2_2) eqn:?; [|congruence].
+  eauto.
+  congruence.
+  congruence.
+Qed.
+
+Lemma GenForall2_bsearch_None_Some : forall A1 A2 (R : A1 -> A2 -> Prop) m1 m2 k a,
+    GenForall2 R m1 m2 ->
+    bsearch k m1 = None ->
+    bsearch k m2 = Some a ->
+    False.
+Proof.
+  intros.
+  destruct H. destruct H.
+  clear H2.
+  revert x m2 H H1.
+  induction m1; intros; simpl in *.
+  destruct a0.
+  destruct m2; [|congruence].
+  destruct p.
+  destruct (Nat.eq_dec n n0); [|congruence].
+  subst.
+  simpl in H1.
+  destruct (k ?= n0) eqn:?.
+  congruence.
+  destruct (zip_map m1_1 m2_1) eqn:?; [|congruence].
+  destruct (zip_map m1_2 m2_2) eqn:?; [|congruence].
+  eauto.
+  destruct (zip_map m1_1 m2_1) eqn:?; [|congruence].
+  destruct (zip_map m1_2 m2_2) eqn:?; [|congruence].
+  eauto.
+  destruct m2.
+  congruence.
+  simpl in *.
+  congruence.
+Qed.
+Inductive Forall2_map A1 A2 (R : A1 -> A2 -> Prop) : tree (nat * A1) -> tree (nat * A2) -> Prop :=
+| FMLeaf : Forall2_map R (Leaf _) (Leaf _)
+| FMNode : forall k a1 a2 l1 l2 r1 r2,
+    R a1 a2 -> Forall2_map R l1 l2 -> Forall2_map R r1 r2 ->
+    Forall2_map R (Node (k, a1) l1 r1) (Node (k, a2) l2 r2).
+
+Lemma GenForall2_Forall2_map : forall A1 A2 (R : A1 -> A2 -> Prop) m1 m2,
+    GenForall2 R m1 m2 <-> Forall2_map R m1 m2.
+Proof.
+  intros.
+  split.
+  revert m2.
+  induction m1; intros.
+  destruct H. destruct H.
+  destruct m2; simpl in *.
+  destruct a.
+  destruct p.
+  destruct (Nat.eq_dec n n0); [|congruence].
+  subst.
+  destruct (zip_map m1_1 m2_1) eqn:?; [|congruence].
+  destruct (zip_map m1_2 m2_2) eqn:?; [|congruence].
+  inversion H.
+  subst.
+  simpl in H0.
+  econstructor.
+  admit.
+  apply IHm1_1.
+  exists t0.
+  split. auto.
+  admit.
+  apply IHm1_2.
+  exists t1.
+  split. auto.
+  admit.
+  destruct a. congruence.
+  destruct H. destruct H.
+  destruct m2.
+  simpl in H. congruence.
+  constructor.
+  revert m2.
+  induction m1; intros.
+  inversion H. subst.
+  apply IHm1_1 in H5.
+  apply IHm1_2 in H6.
+  destruct H5. destruct H0.
+  destruct H6. destruct H2.
+  exists (Node (k,(a1,a2)) x x0).
+  split.
+  simpl.
+  destruct (Nat.eq_dec k k); [|congruence].
+  simpl in H0.
+  rewrite H0.
+  simpl in H2.
+  rewrite H2.
+  auto.
+  simpl.
+  admit.
+  inversion H.
+  subst.
+  exists (Leaf _).
+  split; simpl; auto.
+Admitted.
+
+Lemma GenForall2_bsearch_Some : forall A1 A2 (R : A1 -> A2 -> Prop) m1 m2 k a1 a2,
+    GenForall2 R m1 m2 ->
+    bsearch k m1 = Some a1 ->
+    bsearch k m2 = Some a2 ->
+    R a1 a2.
+Proof.
+  intros.
+  apply GenForall2_Forall2_map in H.
+  revert m2 a1 a2 H H0 H1.
+  induction m1; simpl in *; intros.
+  inversion H. subst.
+  simpl in H1.
+  destruct (k ?= k0) eqn:?.
+  inversion H0. subst.
+  inversion H1. subst.
+  auto.
+  eauto.
+  eauto.
+  congruence.
+Qed.
+
+Lemma GenForall2_bsearch_Some_equiv_coro : forall A B (IA : Inhabit A) (IB : Inhabit B) state (step : step_type (const_yield A) (const_yield B) state) x1 x2 n a1 a2,
+    GenForall2 (fun (coro : coro_type step) (st : state) => equiv_coro' step st coro) x1 x2 ->
+    bsearch n x1 = Some a1 ->
+    bsearch n x2 = Some a2 ->
+    equiv_coro' step a2 a1.
+Proof.
+  intros.
+  eapply (GenForall2_bsearch_Some (R := fun c s => equiv_coro' step s c)).
+  apply H.
+  eauto.
+  eauto.
+Qed.
+
+Hint Resolve GenForall2_bsearch_Some_None GenForall2_bsearch_None_Some GenForall2_bsearch_Some_equiv_coro : foldable.
+
+Definition coro_map_loop fuel :=
+  pipe (ex_coroutine 0)
+       (fun c : coro_type ltac:(let step := get_step (ex_coroutine 0) in exact step) =>
+          nat_rect_nondep
+            (fun _ => Done _ _)
+            (fun _ rec m' =>
+               key <- getN;
+                 option_branch
+                   (fun c : @coro_type nat nat _ _ =>
+                      n <- getN;
+                        r <- resume c $ n;
+                        putN r;
+                        rec (replace_map key c m'))
+                   (rec m')
+                   (bsearch key m'))
+            fuel (Node (0,c) (Leaf _) (Leaf _))).
+
+(*
+Lemma coro_map_loop_ex : forall fuel,
+    coro_map_loop fuel =
+    ltac:(let x := (eval red in (coro_map_loop fuel)) in
+          let x' := coro_to_state x in exact x').
+Proof.
+  intros.
+  unfold coro_map_loop.
+  unfold pipe.
+  generalize_and_ind.
+  reflexivity.
+  f_equal.
+  extensionality key.
+  dest_opt.
+  f_equal.
+  extensionality r.
+  proc_step.
+  eapply GenForall2_bsearch_Some_equiv_coro.
+  eauto.
+  eauto.
+  apply Heqo0.
+  eauto.
+  eauto with typeclass_instances.
+  rewrite <- Heqo0.
+  pattern (bsearch key t1).
+  refine eq_refl.
+  match goal with
+    |- ?lhs = ?rhs =>
+    tryif constr_eq lhs rhs then
+      idtac
+    else
+      fail 0
+  end.
+*)
